Pushing the change through
... including lots of cleanup

ifc/extended/Machine/LabSetsOfPrins.v
@@ -2,7 +2,7 @@ Require Export RelationClasses.
 Require Export SetoidClass.
 Require Import ZArith.
 Require Import ListSet.
-Require Import List.
+Require Import List. Import ListNotations.
 Require Import Bool.
 Require Import Eqdep_dec.
 
@@ -508,3 +508,14 @@ Defined.
 Definition Label := Zset.t.
 Definition label_of_list (l : list Z) :=
   fold_left (fun a b => Zset.add b a) l Zset.empty.
+
+Fixpoint powerset {A : Type} (l : list A) : (list (list A)) :=
+  match l with
+    | [] => [[]]
+    | h::t =>
+      let p := powerset t in
+      map (cons h) p ++ p
+  end.
+
+Definition allThingsBelow (l : Label) :=
+  map label_of_list (powerset (Zset.elements l)).
