ifc/extended/Testing/Common.v
@@ -1,33 +1,18 @@
+Require Import List. Import ListNotations.
+Require Import ZArith.
+Require Import String.
+Require Import NPeano.
+
 Require Import QuickChick Gen.
 
 Require Import Machine.
-
-Require Import List.
-Require Import ZArith.
-Require Import String.
-Require Import Coq.Numbers.Natural.Peano.NPeano.
-
-(* List notations - isn't there a way to import these?! *)
-Notation " [ ] " := nil : list_scope.
-Notation " [ x ] " := (cons x nil) : list_scope.
-Notation " [ x ; .. ; y ] " := (cons x .. (cons y nil) ..) : list_scope.
-
-(* Helper functions *)
-Definition flip {A B C : Type} (f : A -> B -> C) (x : B) (y : A) : C := f y x.
-Definition compose {A B C : Type} (f : B -> C) (g : A -> B) (x : A) : C := f (g x).
-Notation " f << g " := (compose f g) (at level 42). (* F# style, because . *)
+Require Import Lab4.
 
 Section GenUtils.
   Context {Gen : Type -> Type}
           `{GenMonad Gen}.
 
 Definition pure {A : Type} (x : A) : Gen A := returnGen x.
-
-(* This is provided by the interface *)
-(* Definition sequenceGen {A : Type} (ms : list (Gen A)) : Gen (list A) := *)
-(*   fold_right (fun m m' => bindGen m  (fun x =>  *)
-(*                           bindGen m' (fun xs => *)
-(*                           returnGen (x :: xs)))) (pure []) ms. *)
 
 Fixpoint foldGen {A B : Type} (f : A -> B -> Gen A) (l : list B) (a : A)
 : Gen A :=
@@ -38,75 +23,28 @@ Fixpoint foldGen {A B : Type} (f : A -> B -> Gen A) (l : list B) (a : A)
 
 End GenUtils.
 
-(* Variation stuff - should be deleted *)
+(* Variation stuff - should be deleted -- CH: ha? it seems used *)
 Inductive Variation {A : Type} :=
-| Var : Label -> A -> A -> Variation.
+| Var : Lab4 -> A -> A -> Variation.
 
 Class ShrinkV (A : Type) := { shrinkV : @Variation A -> list (@Variation A) }.
 (* End of to be deleted *)
 
-(* List helpers *)
-Fixpoint concat {A : Type} (l : list (list A)) : (list A) :=
-  match l with
-    | [] => []
-    | (h :: t) => h ++ concat t
-  end.
-
-Fixpoint powerset {A : Type} (l : list A) : (list (list A)) :=
-  match l with
-    | [] => [[]]
-    | h::t =>
-      let p := powerset t in
-      map (cons h) p ++ p
-  end.
-
-Fixpoint forallb2 {A : Type} (f : A -> A -> bool) (l1 l2 :list A) : bool :=
-  match l1, l2 with
-    | nil, nil => true
-    | h1::t1, h2::t2 => f h1 h2 && forallb2 f t1 t2
-    | _, _ => false
-  end.
-
-(* Label helpers *)
-Definition lab_of_list (l : list Z) : Label :=
-  fold_left (fun a b => Zset.add b a) l Zset.empty.
-
 (* Short for a label l to be low/high compared to an observability label obs *)
-Definition isLow  (l obs : Label) := flows l obs.
-Definition isHigh (l obs : Label) := negb (isLow l obs).
+Definition isLow  (l obs : Lab4) := flows l obs.
+Definition isHigh (l obs : Lab4) := negb (isLow l obs).
 
-Fixpoint list_of_option {A : Type} (l : list (option A)) : list A :=
-  match l with
-    | nil => nil
-    | Some h :: t => h :: list_of_option t
-    | None :: t => list_of_option t
-  end.
-
-Fixpoint optOfList {A : Type} (l : list (option A)) (acc : list A)
-: option (list A) :=
-  match l with
-    | nil  => Some acc
-    | None::_ => None
-    | Some h :: t => optOfList t (h :: acc)
-  end.
-
-Definition option_bind {X Y} (f : X -> option Y) (o : option X) :=
-  match o with
-  | Some x => f x
-  | None => None
-  end.
-
-Definition validJump (st : State) (addr : Z) :=
-  let '(St imem _ _ _ _ _) := st in
+Definition validJump (st : @State Lab4) (addr : Z) :=
+  let '(St imem _ _ _ _) := st in
   (Z.to_nat addr) <? (List.length imem).
 
-Fixpoint containsRet (stk : Stack) :=
+Fixpoint containsRet (stk : @Stack Lab4) :=
   match stk with
     | Mty => false
     | RetCons _ _ => true
   end.
 
-Definition incr_ptr (p : Pointer) :=
+Definition incr_ptr (p : @Pointer Lab4) :=
   let (fp, i) := p in (Ptr fp (Zsucc i)).
 
 (* Simple equalities *)
@@ -131,14 +69,7 @@ Proof. decide equality. Defined.
 
 Definition instr_eq i1 i2 := if instr_eq_dec i1 i2 then true else false.
 
-Definition label_eq l1 l2 := flows l1 l2 && flows l2 l1.
+Definition label_eq (l1 l2 : Lab4) := flows l1 l2 && flows l2 l1.
 
-Definition indistLabel (l1 l2 : Label) := label_eq l1 l2.
-
-Definition mframe_eq (m1 m2 : mframe) : bool :=
+Definition mframe_eq (m1 m2 : @mframe Lab4) : bool :=
   if Mem.EqDec_block m1 m2 then true else false.
-
-Instance allBelow : AllThingsBelow Label :=
-{|
-  allThingsBelow l := map label_of_list (powerset (Zset.elements l))
-|}.
